feat: implement a notion of well formed expressions + a reflection principle

SSA/Experiment/SSAToTree.lean
@@ -1,21 +1,163 @@
 -- We create a verified conversion from SSA minus Regions (ie, a sequence
 -- of let bindings) into an expression tree. We prove that this
 -- conversion preserves program semantics.
+import Aesop
 
 inductive Kind where
 | int
 | pair : Kind → Kind → Kind
 
-inductive OpKind
+inductive ExprKind
 | O
 | Os
+abbrev Var := String 
 
-inductive Op : OpKind → Type where
-| assign (ret : Var) (kind: OpKind) (arg: Var) : Op .O
-| tuple (ret : Var) (arg1 arg2 : Var) : Op .O
-| ops: Op .O → Op .Os → Op .Os
+inductive OpKind
+| add
+| const
+| sub
 
+inductive Expr : ExprKind → Type where
+| assign (ret : Var) (kind: OpKind) (arg: Var) : Expr .O
+| tuple (ret : Var) (arg1 arg2 : Var) : Expr .O
+| ops: Expr .O → Expr .Os → Expr .Os
+abbrev Op := Expr .O
+abbrev Ops := Expr .Os
+
+@[match_pattern]
+abbrev Op.assign (ret : Var) (kind : OpKind) (arg : Var) : Op := 
+  Expr.assign ret kind arg
+
+@[match_pattern]
+abbrev Op.tuple (ret arg1 arg2: Var) : Op := 
+  Expr.tuple ret arg1 arg2
 
 inductive ExprTree where
 | tuple: ExprTree → ExprTree → ExprTree
-| compute: ExprTree → OpKind → ExprTree
+| compute: ExprTree → ExprKind → ExprTree
+
+-- A DefContext that tracks which variables have been defined.
+def DefContext := String → Bool
+
+abbrev DefContext.bound? (ctx : DefContext) (name : String) : Bool := 
+  ctx name 
+
+abbrev DefContext.bind (ctx : DefContext) (bindname : String) : DefContext := 
+  fun name => if name = bindname then True else ctx name
+
+inductive ExprWellFormed : DefContext → Expr kind → DefContext → Prop where
+| assign
+    {ret arg : Var}
+    {ctx : DefContext}
+    (ARG : ctx.bound? arg = True)
+    (RET: ctx.bound? ret = False) :
+    ExprWellFormed ctx (Op.assign ret kind arg) (ctx.bind ret)
+| tuple
+  {ctx : DefContext}
+  {ret arg1 arg2 : Var}
+  (ARG1 : ctx.bound? arg1 = True)
+  (ARG2 : ctx.bound? arg2 = True)
+  (RET: ctx.bound? ret = False) :
+  ExprWellFormed ctx (Op.tuple ret arg1 arg2) (ctx.bind ret)
+| ops 
+  {ctxbegin ctxend : DefContext}
+  ⦃ctxmid : DefContext⦄
+  (WF1: ExprWellFormed ctxbegin op1 ctxmid)
+  (WF2: ExprWellFormed ctxmid op2 ctxend) : 
+  ExprWellFormed ctxbegin (Expr.ops op1 op2) ctxend
+
+def ExprWellFormed.compute : Expr kind → DefContext → Option DefContext 
+| (.assign ret kind arg), ctx => 
+    if ctx.bound? ret 
+    then .none
+    else if not (ctx.bound? arg)
+    then .none
+    else .some (ctx.bind ret)
+| (.tuple ret arg1 arg2), ctx => 
+    if ctx.bound? ret then .none
+    else if not (ctx.bound? arg1) then .none
+    else if not (ctx.bound? arg2) then .none
+    else .some (ctx.bind ret)
+| (Expr.ops op1 op2), ctx => 
+    Option.bind (ExprWellFormed.compute op1 ctx) (ExprWellFormed.compute op2)
+
+-- (compute = true) => (stuff holds)
+theorem ExprWellFormed.compute_implies_prop:
+  ∀ (ctx ctx' : DefContext) (expr : Expr kind),
+  .some ctx' = ExprWellFormed.compute expr ctx -> 
+  ExprWellFormed ctx expr ctx' := by {
+  intros ctx ctx' expr;
+  revert ctx ctx';
+  induction expr;
+  case assign ret kind arg => {
+    intros ctx ctx' COMPUTE;
+    simp[compute] at COMPUTE;
+    aesop; constructor <;> aesop;
+  }
+  case tuple ret arg1 arg2 => {
+    intros ctx ctx' COMPUTE;
+    simp[compute] at COMPUTE;
+    aesop; constructor <;> aesop;
+  }
+  case ops o1 o2 IH1 IH2 => {
+    intros ctx ctx'' COMPUTE;
+    simp[compute] at COMPUTE;
+    cases CTXO1:(compute o1 ctx) <;> simp[CTXO1] at COMPUTE; case some ctx' => {
+      cases CTXO2:(compute o2 ctx') <;> simp[CTXO2] at COMPUTE; case some ctx''_2 => {
+       -- | TODO @chris: how to write this nicer, to prevent the induction COMPUTE;
+        induction COMPUTE; case refl => { 
+          apply ExprWellFormed.ops (ctxmid := ctx') <;> aesop;
+        }
+      }
+    }
+  }
+}
+
+theorem ExprWellFormed.prop_implies_compute:
+  ∀ (ctx ctx' : DefContext) (expr : Expr kind),
+  ExprWellFormed ctx expr ctx' -> 
+  .some ctx' = ExprWellFormed.compute expr ctx := by {
+  intros ctx ctx' expr;
+  revert ctx ctx';
+  induction expr;
+  case assign ret kind arg => {
+    intros ctx ctx' WELLFORMED;
+    cases WELLFORMED;
+    case assign RET ARG => {
+      simp[compute]; aesop;
+    }
+  }
+  case tuple ret arg1 arg2 => {
+    intros ctx ctx' WELLFORMED;
+    cases WELLFORMED;
+    case tuple RET ARG1 ARG2 => {
+      simp[compute]; aesop;
+    }
+  }
+  case ops op1 op2 IH1 IH2 => {
+    intros ctx ctx'' WELLFORMED;
+    cases WELLFORMED;
+    case ops ctx' WF1 WF2 => {
+      simp[compute];
+      specialize (IH1 _ _ WF1);
+      specialize (IH2 _ _ WF2);
+      cases OP1:(compute op1 ctx) <;> simp[OP1] at IH1;
+      cases OP2:(compute op2 ctx') <;> simp[OP2] at IH2;
+      aesop;
+    }
+  }
+}
+
+-- Reflection tactic to reflect the proof level 'ExprWellFormed'
+-- into computation level 'ExprWellFormed.compute'
+theorem ExprWellFormed.reflect : 
+  ∀ (ctx ctx' : DefContext) (expr : Expr kind),
+  .some ctx' = ExprWellFormed.compute expr ctx <-> 
+  ExprWellFormed ctx expr ctx' := by {
+  intros ctx ctx' expr; 
+  constructor
+  case mp => { apply ExprWellFormed.compute_implies_prop; }
+  case mpr => { apply ExprWellFormed.prop_implies_compute; }
+}
+
+
